lean/LeanTs.lean
@@ -11,6 +11,7 @@ import LeanTs.Vectors
 import LeanTs.Builder
 import LeanTs.Syntax
 import LeanTs.Ident
+import LeanTs.Parse
 import LeanTs.JsSem
 import LeanTs.Agree
 import LeanTs.Exhaustive
